pancake/semantics/panSemScript.sml
@@ -719,7 +719,12 @@ Definition evaluate_decls_def:
           NONE)
    | NONE => NONE) ∧
   evaluate_decls s (Function fi::ds) =
-  evaluate_decls (s with code := s.code |+ (fi.name,(fi.params,fi.body))) ds
+  evaluate_decls (s with code := s.code |+ (fi.name,(fi.params,fi.body))) ds ∧
+  evaluate_decls s (EidDecl eid sh :: ds) = 
+    if FLOOKUP s.eshapes eid = NONE then
+      evaluate_decls (s with eshapes := s.eshapes |+ (eid, sh)) ds
+    else
+      NONE
 End
 
 Definition semantics_decls_def:
